Refactored spec_locks/verif_locks, created test/verif_incr

lib/proof/spec_locks.v
@@ -1,9 +1,9 @@
 Require Import VST.veric.rmaps.
 Require Import VST.concurrency.conclib.
-Require Import locks.
-Require Import spec_malloc.
-(* Require Import VST.floyd.library.
-*)
+Require Import VST.concurrency.cancelable_invariants.
+Require Import VST.concurrency.ghosts. 
+Require Import VSTlib.locks.
+Require Import VSTlib.spec_malloc.
 Import FashNotation.
 
 (* lock invariants should be exclusive *)
@@ -143,21 +143,103 @@ Proof.
   apply data_at__data_at; eauto.
 Qed.
 
+Definition lock_handle : Type := val * invariants.iname * ghosts.gname.
+
+Definition ptr_of (h: lock_handle) : val := let '(v, i, g) := h in v.
+
+  (* We can use self_part sh h * R instead of selflock sh h R. *)
+Definition self_part sh (h : val * invariants.iname * ghosts.gname) := let '(v, i, g) := h in cinv_own g sh.
+
+Lemma self_part_exclusive : forall sh h, sh <> Share.bot -> exclusive_mpred (self_part sh h).
+  Proof.
+    intros; unfold exclusive_mpred, self_part; destruct h as ((?, ?), ?).
+    unfold cinv_own; rewrite own_op'; Intros ?.
+    apply sepalg.join_self, identity_share_bot in H0; contradiction.
+  Qed.
+
+#[export] Hint Resolve self_part_exclusive : core.
+
+
 Class lockAPD := {
   t_lock : type := Tstruct _atom_int noattr;
-  lock_handle : Type;
-  ptr_of : lock_handle -> val;
-  lock_inv : share -> lock_handle -> mpred -> mpred;
-  lock_inv_nonexpansive : forall sh h, nonexpansive (lock_inv sh h);
-  lock_inv_share_join : forall sh1 sh2 sh3 h R, sh1 <> Share.bot -> sh2 <> Share.bot ->
-    sepalg.join sh1 sh2 sh3 -> lock_inv sh1 h R * lock_inv sh2 h R = lock_inv sh3 h R;
-  lock_inv_exclusive : forall sh h R, exclusive_mpred (lock_inv sh h R);
-  lock_inv_isptr : forall sh h R, lock_inv sh h R |-- !! isptr (ptr_of h) 
+  inv_for_lock: forall (v: val) (R: mpred), mpred;
+  inv_for_lock_nonexpansive : forall v, nonexpansive (inv_for_lock v)
 }.
+
+Definition lock_inv {L: lockAPD} (sh: share) (h: lock_handle)  (R: mpred) :=
+   let '(v, i, g) := h in !!(sh <> Share.bot /\ isptr v) && cinvariant i g (inv_for_lock v R) * cinv_own g sh.
+
+Lemma lock_inv_nonexpansive {L: lockAPD}  : forall sh h, nonexpansive (lock_inv sh h).
+  Proof.
+   intros.
+    unfold lock_inv. destruct h as [[? ?] ?].
+    apply sepcon_nonexpansive, const_nonexpansive.
+    apply @conj_nonexpansive; [apply const_nonexpansive|].
+    apply cinvariant_nonexpansive2, inv_for_lock_nonexpansive.
+  Qed.
+
+Lemma lock_inv_share_join {L: lockAPD} : forall sh1 sh2 sh3 h R, sh1 <> Share.bot -> sh2 <> Share.bot ->
+    sepalg.join sh1 sh2 sh3 -> lock_inv sh1 h R * lock_inv sh2 h R = lock_inv sh3 h R.
+  Proof.
+    unfold lock_inv. destruct h as [[??]?]. intros.
+    destruct (isptr_dec v).
+    rewrite !prop_true_andp; auto.
+    rewrite <- !sepcon_assoc, (sepcon_comm (_ * cinv_own _ _)), !sepcon_assoc.
+    unfold cinv_own at 1 2; erewrite <- own_op by eauto.
+    rewrite <- sepcon_assoc; f_equal.
+    symmetry; apply cinvariant_dup.
+    { split; auto; intros ?; subst. apply join_Bot in H1 as []; contradiction. }
+    { rewrite prop_false_andp, !FF_sepcon, prop_false_andp, FF_sepcon; auto; intros []; contradiction. }
+  Qed.
+
+Lemma lock_inv_exclusive  {L: lockAPD} : forall sh h R, exclusive_mpred (lock_inv sh h R).
+  Proof.
+    intros. destruct h as [[??]?].
+    unfold exclusive_mpred, lock_inv; Intros.
+    unfold cinv_own. sep_apply @own_op'.
+    Intros ?; Intros.
+    apply sepalg.join_self, identity_share_bot in H0; contradiction.
+  Qed.
+
+Lemma lock_inv_share  {L: lockAPD} : forall sh h R, lock_inv sh h R |-- !!(sh <> Share.bot /\ isptr (ptr_of h)).
+  Proof.
+    intros.
+    unfold lock_inv. destruct h as [[??]?]. entailer!. 
+Qed.
+
+#[export] Hint Resolve lock_inv_share : saturate_local.
+
+#[export] Hint Resolve lock_inv_exclusive data_at_exclusive data_at__exclusive field_at_exclusive field_at__exclusive : core.
+
+Lemma self_part_eq  {L: lockAPD} : forall 
+    (sh1 sh2: share)
+   (h: val * invariants.iname * ghosts.gname) R, 
+   sh2 <> Share.bot -> 
+    lock_inv sh1 h (self_part sh2 h * R) * self_part sh2 h =
+    lock_inv sh1 h (self_part sh2 h * R) * lock_inv sh2 h (self_part sh2 h * R).
+  Proof.
+    intros.
+    simpl; unfold self_part, lock_inv; destruct h as ((?, ?), ?).
+    destruct (eq_dec sh1 Share.bot).
+    { rewrite prop_false_andp, !FF_sepcon; auto; intros []; contradiction. }
+    destruct (isptr_dec v).
+    rewrite !prop_true_andp by auto.
+    rewrite cinvariant_dup at 1.
+    rewrite <- !sepcon_assoc; f_equal.
+    rewrite (sepcon_comm (_ * _) (cinvariant _ _ _)), <- sepcon_assoc; reflexivity.
+    { rewrite prop_false_andp, !FF_sepcon; auto; intros []; contradiction. }
+  Qed.
+
+Ltac lock_props := match goal with |-context[weak_exclusive_mpred ?P && emp] => sep_apply (exclusive_weak_exclusive P); [auto with share | try timeout 20 cancel] end.
 
 Section lock_specs.
 
   Context {M: MallocAPD} {L : lockAPD}.
+
+  Definition selflock R sh h := self_part sh h * R.
+
+  Lemma lock_inv_isptr : forall sh h R, lock_inv sh h R |-- !! isptr (ptr_of h).
+  Proof. intros. entailer!. Qed.
 
   Lemma lock_inv_nonexpansive2 : forall {A} (P Q : A -> mpred) sh p x, (ALL x : _, |> (P x <=> Q x) |--
     |> lock_inv sh p (P x) <=> |> lock_inv sh p (Q x))%logic.
@@ -165,7 +247,7 @@ Section lock_specs.
     intros.
     apply allp_left with x.
     eapply derives_trans, eqp_later1; apply later_derives.
-    apply nonexpansive_entail; apply L.(lock_inv_nonexpansive).
+    apply nonexpansive_entail; apply lock_inv_nonexpansive.
   Qed.
 
   Lemma lock_inv_super_non_expansive : forall sh h R n,
@@ -385,6 +467,109 @@ Section lock_specs.
     apply wand_refl_cancel_right.
   Qed.
 
+(* freelock and release specialized for self_part *)
+Program Definition freelock_spec_self :=
+  TYPE (ProdType (ConstType _) Mpred)
+  WITH sh1 : _, sh2 : _, h : _, R : _
+  PRE [ tptr t_lock ]
+     PROP (sh2 <> Share.bot; sepalg.join sh1 sh2 Tsh)
+     PARAMS (ptr_of h)
+     SEP (lock_inv sh1 h (self_part sh2 h * R); self_part sh2 h)
+  POST [ tvoid ]
+     PROP ()
+     LOCAL ()
+     SEP ().
+Next Obligation.
+Proof.
+  repeat intro.
+  destruct x as (((?, ?), ?), ?); simpl.
+  unfold PROPx, PARAMSx, GLOBALSx, LOCALx, SEPx, argsassert2assert; simpl; rewrite !approx_andp; do 3 f_equal;
+    rewrite -> !sepcon_emp, ?approx_sepcon, ?approx_idem.
+  f_equal.
+  setoid_rewrite lock_inv_super_non_expansive; do 2 f_equal.
+  rewrite !approx_sepcon, approx_idem; auto.
+Qed.
+Next Obligation.
+Proof.
+  repeat intro.
+  destruct x as (((?, ?), ?), ?); simpl.
+  unfold PROPx, LOCALx, SEPx; simpl; rewrite !approx_andp; do 2 f_equal;
+    rewrite -> !sepcon_emp, ?approx_sepcon, ?approx_idem.
+Qed.
+
+Program Definition release_spec_self :=
+  TYPE (ProdType (ConstType _) Mpred)
+  WITH sh : _, h : _, R : _
+  PRE [ tptr t_lock ]
+     PROP ()
+     PARAMS (ptr_of h)
+     SEP (lock_inv sh h (self_part sh h * R); R)
+  POST [ tvoid ]
+     PROP ()
+     LOCAL ()
+     SEP ().
+Next Obligation.
+Proof.
+  repeat intro.
+  destruct x as ((?, ?), ?); simpl.
+  unfold PROPx, PARAMSx, GLOBALSx, LOCALx, SEPx, argsassert2assert; simpl; rewrite !approx_andp; do 3 f_equal;
+    rewrite -> !sepcon_emp, ?approx_sepcon, ?approx_idem.
+  f_equal.
+  setoid_rewrite lock_inv_super_non_expansive; do 2 f_equal.
+  rewrite !approx_sepcon, approx_idem; auto.
+Qed.
+Next Obligation.
+Proof.
+  repeat intro.
+  destruct x as ((?, ?), ?); simpl.
+  reflexivity.
+Qed.
+
+Lemma release_self : funspec_sub release_spec release_spec_self.
+Proof.
+  unfold funspec_sub; simpl.
+  split; auto; intros ? ((sh, h), R) ?; Intros.
+  eapply derives_trans, fupd_intro.
+  Exists (nil : list Type) (sh, h, self_part sh h * R, R, emp) emp; entailer!.
+  { intros; unfold PROPx, LOCALx, SEPx; simpl; entailer!. }
+  unfold lock_inv; destruct h as ((?, ?), ?).
+  unfold PROPx, PARAMSx, GLOBALSx, LOCALx, SEPx, argsassert2assert; simpl; entailer!.
+  lock_props.
+  { apply exclusive_sepcon1.
+     apply (self_part_exclusive sh (v,i,g)); auto.
+ }
+  rewrite <- sepcon_emp at 1; apply sepcon_derives; [apply now_later|].
+  rewrite <- wand_sepcon_adjoint, emp_sepcon; cancel.
+  apply inv_dealloc.
+Qed.
+
+Lemma freelock_self : funspec_sub freelock_spec freelock_spec_self.
+Proof.
+  unfold freelock_spec, freelock_spec_self.
+  unfold funspec_sub; simpl.
+  split; auto; intros ? (((sh1, sh2), h), R) ?; Intros.
+  eapply derives_trans, fupd_intro.
+  Exists (nil : list Type) (h, self_part sh2 h * R, emp) emp; entailer!.
+  { intros; unfold PROPx, LOCALx, SEPx; simpl; entailer!. }
+  unfold PROPx, PARAMSx, GLOBALSx, LOCALx, SEPx, argsassert2assert; simpl.
+  set (P := _ * _); entailer!; subst P.
+  rewrite sepcon_emp; setoid_rewrite self_part_eq; auto.
+  saturate_local.
+  erewrite lock_inv_share_join by eauto; simpl; cancel.
+  apply andp_right; auto.
+  rewrite <- wand_sepcon_adjoint, emp_sepcon.
+  destruct h as ((p, i), g); simpl; Intros.
+  sep_apply cinv_own_excl.
+  rewrite FF_sepcon; auto.
+Qed.
+
+Opaque lock_handle.
+Opaque ptr_of.
+Opaque lock_inv.
+Opaque self_part.
+Arguments ptr_of : simpl never.
+Arguments lock_inv : simpl never.
+
 Definition LockASI:funspecs := [
    (_makelock, makelock_spec);
    (_freelock, freelock_spec);
@@ -393,8 +578,3 @@ Definition LockASI:funspecs := [
 ].
 
 End lock_specs.
-
-#[export] Hint Resolve lock_inv_isptr : saturate_local.
-#[export] Hint Resolve lock_inv_exclusive data_at_exclusive data_at__exclusive field_at_exclusive field_at__exclusive : core.
-
-Ltac lock_props := match goal with |-context[weak_exclusive_mpred ?P && emp] => sep_apply (exclusive_weak_exclusive P); [auto with share | try timeout 20 cancel] end.
